theories/case_studies/vae/vae.v
@@ -1,7 +1,7 @@
 From iris.algebra Require Import frac.
 From iris.proofmode Require Import proofmode.
 From cap_machine Require Import rules proofmode.
-From cap_machine Require Import fetch assert.
+From cap_machine Require Import fetch assert switcher.
 
 Section VAE_Main.
   Context `{MP: MachineParameters}.
@@ -101,7 +101,7 @@ Section VAE_Main.
       (vae_main_imports za za za za_ot za za (SCap RO Global za za za)).
 
   Definition vae_exp_tbl_entry_awkward :=
-    WInt (switcher.encode_entry_point 1
+    WInt (encode_entry_point 1
             (length_vae_main_imports + (length VAE_main_code_init))).
 
   Definition vae_entry_awkward_sb
