theories/logrel/ftlr/BinOp.v
@@ -17,7 +17,6 @@ Section fundamental.
     {cstackg : CSTACKG Σ}
     {nainv: logrel_na_invs Σ}
     `{MP: MachineParameters}
-    {swlayout : switcherLayout}
   .
 
   Implicit Types W : WORLD.
@@ -30,8 +29,7 @@ Section fundamental.
 
   Lemma binop_case (W : WORLD) (C : CmptName) (regs : leibnizO Reg) (p p' : Perm)
     (g : Locality) (b e a : Addr) (w : Word) (ρ : region_type) (dst : RegName)
-    (r1 r2: Z + RegName) (P:D) (cstk : CSTK) (Ws : list WORLD) (Cs : list CmptName) (wstk : Word)
-    (Nswitcher : namespace) :
+    (r1 r2: Z + RegName) (P:D) (cstk : CSTK) (Ws : list WORLD) (Cs : list CmptName) :
     ftlr_instr_base W C regs p p' g b e a w ρ P
       (decodeInstrW w = Add dst r1 r2 \/
        decodeInstrW w = Sub dst r1 r2 \/
@@ -41,11 +39,11 @@ Section fundamental.
        decodeInstrW w = LShiftL dst r1 r2 \/
        decodeInstrW w = LShiftR dst r1 r2 \/
        decodeInstrW w = Lt dst r1 r2
-      ) cstk Ws Cs wstk Nswitcher.
+      ) cstk Ws Cs.
   Proof.
     intros Hp Hsome HcorrectPC Hbae Hfp HO Hpers Hpwl Hregion Hnotrevoked Hi.
     iIntros "#IH #Hinv_interp #Hreg #Hinva #Hrcond #Hwcond #Hmono #HmonoV Hw Hcont %Hframe Hsts Hown Htframe".
-    iIntros "Hr Hstate Ha HPC Hmap %Hsp #Hswitcher".
+    iIntros "Hr Hstate Ha HPC Hmap".
     iInsert "Hmap" PC.
 
     iApply (wp_BinOp with "[$Ha $Hmap]"); eauto.
@@ -66,7 +64,7 @@ Section fundamental.
 
       assert (is_Some (<[dst:=WInt (rules_BinOp.denote (decodeInstrW w) n1 n2)]> (<[PC:=WCap x x0 x1 x2 x3]> regs) !! csp)) as [??].
       { destruct (decide (dst = csp)); simplify_map_eq=>//. }
-      iApply ("IH" $! _ _ _ _ _ (<[dst:=_]> (<[PC:=_]> regs)) with "[%] [] [Hmap] [%] [$Hr] [$Hsts] [$Hcont] [//] [$Hown] [$Htframe]")
+      iApply ("IH" $! _ _ _ _ _ (<[dst:=_]> (<[PC:=_]> regs)) with "[%] [] [Hmap] [$Hr] [$Hsts] [$Hcont] [//] [$Hown] [$Htframe]")
       ; eauto.
       + intro; cbn. by repeat (rewrite lookup_insert_is_Some'; right).
       + iIntros (ri wi Hri Hregs_ri).
