theories/logrel/ftlr/Mov.v
@@ -16,7 +16,6 @@ Section fundamental.
     {cstackg : CSTACKG Σ}
     {nainv: logrel_na_invs Σ}
     `{MP: MachineParameters}
-    {swlayout : switcherLayout}
   .
 
   Implicit Types W : WORLD.
@@ -29,13 +28,12 @@ Section fundamental.
 
    Lemma mov_case (W : WORLD) (C : CmptName) (regs : leibnizO Reg)
      (p p' : Perm) (g : Locality) (b e a : Addr)
-     (w : Word) (ρ : region_type) (dst : RegName) (src : Z + RegName) (P:D) (cstk : CSTK) (Ws : list WORLD) (Cs : list CmptName) (wstk : Word)
-     (Nswitcher : namespace) :
-    ftlr_instr W C regs p p' g b e a w (Mov dst src) ρ P cstk Ws Cs wstk Nswitcher.
+     (w : Word) (ρ : region_type) (dst : RegName) (src : Z + RegName) (P:D) (cstk : CSTK) (Ws : list WORLD) (Cs : list CmptName) :
+    ftlr_instr W C regs p p' g b e a w (Mov dst src) ρ P cstk Ws Cs.
   Proof.
     intros Hp Hsome HcorrectPC Hbae Hfp HO Hpers Hpwl Hregion Hnotrevoked Hi.
     iIntros "#IH #Hinv_interp #Hreg #Hinva #Hrcond #Hwcond #Hmono #HmonoV Hw Hcont %Hframe Hsts Hown Htframe".
-    iIntros "Hr Hstate Ha HPC Hmap %Hsp #Hswitcher".
+    iIntros "Hr Hstate Ha HPC Hmap".
     iInsert "Hmap" PC.
     iApply (wp_Mov with "[$Ha $Hmap]"); eauto.
     { simplify_map_eq; auto. }
@@ -62,7 +60,7 @@ Section fundamental.
         { destruct ρ;auto;contradiction. }
         destruct (decide (r = PC)).
         { simplify_map_eq.
-          iApply ("IH" $! _ _ _ _ _ regs with "[%] [] [Hmap] [%] [$Hr] [$Hsts] [$Hcont] [//] [$Hown] [$Htframe]"); eauto.
+          iApply ("IH" $! _ _ _ _ _ regs with "[%] [] [Hmap] [$Hr] [$Hsts] [$Hcont] [//] [$Hown] [$Htframe]"); eauto.
           iApply (interp_next_PC with "Hinv_interp"); eauto.
         }
         simplify_map_eq.
@@ -76,7 +74,7 @@ Section fundamental.
           iApply wp_value;auto.
         }
 
-        iApply ("IH" $! _ _ _ _ _ regs with "[%] [] [Hmap] [%] [$Hr] [$Hsts] [$Hcont] [//] [$Hown] [$Htframe]"); eauto.
+        iApply ("IH" $! _ _ _ _ _ regs with "[%] [] [Hmap] [$Hr] [$Hsts] [$Hcont] [//] [$Hown] [$Htframe]"); eauto.
         iApply (interp_weakening with "IH Hr0"); eauto; try reflexivity; try solve_addr.
       }
       { map_simpl "Hmap".
@@ -84,7 +82,7 @@ Section fundamental.
         { destruct ρ;auto;contradiction. }
         assert (is_Some (<[dst:=w0]> regs !! csp)) as [??].
         { destruct (decide (dst = csp));simplify_map_eq =>//. }
-        iApply ("IH" $! _ _ _ _ _ (<[dst:=w0]> _) with "[%] [] [Hmap] [//] [$Hr] [$Hsts] [$Hcont] [//] [$Hown] [$Htframe]"); eauto.
+        iApply ("IH" $! _ _ _ _ _ (<[dst:=w0]> _) with "[%] [] [Hmap] [$Hr] [$Hsts] [$Hcont] [//] [$Hown] [$Htframe]"); eauto.
         - intros; simpl.
           rewrite lookup_insert_is_Some.
           destruct (decide (dst = x0)); auto; right; split; auto.
