theories/logrel/ftlr/interp_weakening.v
@@ -13,13 +13,12 @@ Section fundamental.
     {nainv: logrel_na_invs Σ}
     {cstackg : CSTACKG Σ}
     `{MP: MachineParameters}
-    {swlayout : switcherLayout}
   .
 
   Implicit Types W : WORLD.
   Implicit Types C : CmptName.
 
-  Notation E := (CSTK -n> list WORLD -n> WORLD -n> (leibnizO CmptName) -n> (leibnizO Word) -n> (leibnizO Word) -n> iPropO Σ).
+  Notation E := (CSTK -n> list WORLD -n> WORLD -n> (leibnizO CmptName) -n> (leibnizO Word) -n> iPropO Σ).
   Notation V := (WORLD -n> (leibnizO CmptName) -n> (leibnizO Word) -n> iPropO Σ).
   Notation R := (WORLD -n> (leibnizO CmptName) -n> (leibnizO Reg) -n> iPropO Σ).
   Implicit Types w : (leibnizO Word).
@@ -31,7 +30,7 @@ Section fundamental.
   Proof.
     iIntros "#Hinterp".
     rewrite /enter_cond /interp_expr /=.
-    iIntros (stk Ws Cs wstk W' Hrelated).
+    iIntros (W' Hrelated).
     iAssert (future_world Global W W')%I as "%Hrelated'".
     { iPureIntro.
       apply related_sts_pub_priv_trans_world with W', related_sts_priv_refl_world; auto.
@@ -39,7 +38,7 @@ Section fundamental.
     iIntros "!> %g' %Hflows".
     assert (  LocalityFlowsTo g' Global ) as Hflow'.
     { destruct g'; auto. }
-    iSpecialize ("Hinterp" $! stk Ws Cs wstk W' Hrelated' g' Hflow').
+    iSpecialize ("Hinterp" $! W' Hrelated' g' Hflow').
     iFrame "#".
   Qed.
 
@@ -157,10 +156,10 @@ Section fundamental.
     iDestruct "HA" as "[#A %Hpwl_cond]".
     iModIntro.
     rewrite /enter_cond /interp_expr /=.
-    iIntros (stk Ws Cs wstk W') "#Hfuture %g'' %Hflows !>".
-    iIntros (regs) "[[Hfull Hmap] (Hreg & Hregion & Hsts & Hcont & Hown & Hframe & Hcstk & %)]".
+    iIntros (W') "#Hfuture %g'' %Hflows !>".
+    iIntros (cstk Ws Cs regs) "[[Hfull Hmap] (Hreg & Hregion & Hsts & Hcont & Hown & Hcstk & Hframe)]".
     rewrite /interp_conf.
-    iApply ("IH" with "Hfull Hmap Hreg Hregion Hsts Hcont Hown [] Hframe Hcstk"); eauto.
+    iApply ("IH" with "Hfull Hmap Hreg Hregion Hsts Hcont Hframe Hown Hcstk"); eauto.
     iModIntro. rewrite fixpoint_interp1_eq interp1_eq.
     destruct (isO p) eqn:HpO; auto.
     destruct (has_sreg_access p) eqn:HpXSR'; auto.
