theories/logrel/monotone.v
@@ -13,15 +13,14 @@ Section monotone.
     {nainv: logrel_na_invs Σ}
     {cstackg : CSTACKG Σ}
     `{MP: MachineParameters}
-    {swlayout : switcherLayout}
   .
 
   Implicit Types W : WORLD.
   Implicit Types C : CmptName.
 
-  Notation E := (CSTK -n> list WORLD -n> leibnizO (list CmptName) -n> WORLD -n> (leibnizO CmptName) -n> (leibnizO Word) -n> (leibnizO Word) -n> iPropO Σ).
+  Notation E := (WORLD -n> (leibnizO CmptName) -n> (leibnizO Word) -n> iPropO Σ).
   Notation V := (WORLD -n> (leibnizO CmptName) -n> (leibnizO Word) -n> iPropO Σ).
-  Notation K := (iPropO Σ).
+  Notation K := (CSTK -n> list WORLD -n> leibnizO (list CmptName) -n> iPropO Σ).
   Notation R := (WORLD -n> (leibnizO CmptName) -n> (leibnizO Reg) -n> iPropO Σ).
   Implicit Types w : (leibnizO Word).
   Implicit Types interp : (V).
@@ -60,7 +59,7 @@ Section monotone.
     intros Hrelated Hstate.
     destruct Hrelated as [ [Hdom_sta Hrelated ] _]. simpl in *.
     assert (is_Some ((std W') !! a)) as [y Hy].
-    { apply Hdom_sta in Hstate; auto. }
+{ rewrite -elem_of_dom. apply elem_of_subseteq in Hdom_sta. apply Hdom_sta. rewrite elem_of_dom;eauto. }
     specialize (Hrelated a Permanent y Hstate Hy).
     eapply std_rel_rtc_Permanent in Hrelated;subst;auto.
   Qed.
@@ -242,7 +241,7 @@ Section monotone.
   Proof.
     iIntros (Hrelated) "#Hw".
     rewrite !fixpoint_interp1_eq /=.
-    iModIntro. iIntros (stk r Ws Cs W'').
+    iModIntro. iIntros (W'').
     destruct g.
     + iIntros "#Hrelated'".
       rewrite /future_world.
@@ -250,7 +249,7 @@ Section monotone.
       iAssert (future_world Global W W'')%I as "Hrelated".
       { rewrite /future_world.
         iPureIntro. apply related_sts_pub_priv_trans_world with W'; auto. }
-      iSpecialize ("Hw" $! stk r Ws Cs W'' with "Hrelated").
+      iSpecialize ("Hw" $! W'' with "Hrelated").
       iApply "Hw".
     + iIntros "#Hrelated'".
       rewrite /future_world.
@@ -258,7 +257,7 @@ Section monotone.
       iAssert (future_world Local W W'')%I as "Hrelated".
       { rewrite /future_world.
         iPureIntro. apply related_sts_pub_trans_world with W'; auto. }
-      iSpecialize ("Hw" $! stk r Ws Cs W'' with "Hrelated").
+      iSpecialize ("Hw" $! W'' with "Hrelated").
       iApply "Hw".
   Qed.
 
@@ -352,14 +351,14 @@ Section monotone.
     iIntros (Hrelated Hnl) "#Hw".
     rewrite !fixpoint_interp1_eq /=.
     destruct g ; cbn in Hnl ; try done.
-    iModIntro. iIntros (stk r Ws Cs W'').
+    iModIntro. iIntros (W'').
     iIntros "#Hrelated'".
     rewrite /future_world.
     iDestruct "Hrelated'" as "%Hrelated'".
     iAssert (future_world Global W W'')%I as "Hrelated".
     { rewrite /future_world.
       iPureIntro. apply related_sts_priv_trans_world with W'; auto. }
-    iSpecialize ("Hw" $! stk r Ws Cs W'' with "Hrelated").
+    iSpecialize ("Hw" $! W'' with "Hrelated").
     iApply "Hw".
   Qed.
 
