theories/switcher/interp_switcher_call.v
@@ -6,6 +6,7 @@ From cap_machine Require Import interp_weakening.
 From cap_machine Require Import wp_rules_interp switcher_macros_spec.
 From cap_machine Require Import rules proofmode monotone.
 From cap_machine Require Import fundamental.
+From cap_machine Require Import switcher_preamble.
 From cap_machine.proofmode Require Import map_simpl register_tactics proofmode.
 
 
@@ -23,23 +24,20 @@ Section fundamental.
   Implicit Types W : WORLD.
   Implicit Types C : CmptName.
 
-  Notation E := (WORLD -n> (leibnizO CmptName) -n> (leibnizO Word) -n> (leibnizO Word) -n> iPropO Σ).
+  Notation E := (WORLD -n> (leibnizO CmptName) -n> (leibnizO Word) -n> iPropO Σ).
   Notation V := (WORLD -n> (leibnizO CmptName) -n> (leibnizO Word) -n> iPropO Σ).
-  Notation K := (WORLD -n> (leibnizO CmptName) -n> iPropO Σ).
+  Notation K := (CSTK -n> list WORLD -n> leibnizO (list CmptName) -n> iPropO Σ).
   Notation R := (WORLD -n> (leibnizO CmptName) -n> (leibnizO Reg) -n> iPropO Σ).
   Implicit Types w : (leibnizO Word).
   Implicit Types interp : (V).
 
-  Lemma interp_expr_switcher_call (W : WORLD) (C : CmptName)
-    (cstk : CSTK) (Ws : list WORLD) (Cs : list CmptName) (wstk : Word)
-    (Nswitcher : namespace)
-    :
+  Lemma interp_expr_switcher_call (W : WORLD) (C : CmptName) (Nswitcher : namespace) :
     na_inv logrel_nais Nswitcher switcher_inv
-    ⊢ interp_expr interp (interp_cont interp cstk Ws Cs) cstk Ws Cs W C (WCap XSRW_ Local b_switcher e_switcher a_switcher_call) wstk.
+    ⊢ interp_expr interp (interp_cont interp) W C (WCap XSRW_ Local b_switcher e_switcher a_switcher_call).
   Proof.
-    iIntros  "#Hinv_switcher %regs [[%Hfull_rmap #Hreg] (Hrmap & %Hstk & Hr & Hsts & Hcont & Hna & Hcstk & %Hframe)]".
+    iIntros "#Hinv_switcher %cstk %Ws %Cs %regs [[%Hfull_rmap #Hreg] (Hrmap & Hr & Hsts & Hcont & Hna & Hcstk & %Hframe)]".
     rewrite /registers_pointsto.
-    iPoseProof (fundamental_ih with "Hinv_switcher") as "IH". (* used for weakening lemma later *)
+    iPoseProof fundamental_ih as "IH". (* used for weakening lemma later *)
 
     (* --- Extract the code from the invariant --- *)
     iMod (na_inv_acc with "Hinv_switcher Hna")
@@ -55,7 +53,7 @@ Section fundamental.
     iHide "Hinv_switcher" as hinv_switcher.
 
     iExtract "Hrmap" PC as "HPC".
-    iExtract "Hrmap" csp as "Hcsp".
+    specialize (Hfull_rmap csp) as HH;destruct HH as [Hstk wcsp].
     specialize (Hfull_rmap cs0) as HH;destruct HH as [? ?].
     specialize (Hfull_rmap cs1) as HH;destruct HH as [? ?].
     specialize (Hfull_rmap cra) as HH;destruct HH as [? ?].
@@ -63,6 +61,7 @@ Section fundamental.
     specialize (Hfull_rmap ct2) as HH;destruct HH as [? ?].
     specialize (Hfull_rmap ctp) as HH;destruct HH as [? ?].
     specialize (Hfull_rmap ct1) as HH;destruct HH as [? ?].
+    iExtract "Hrmap" csp as "Hcsp".
     iExtract "Hrmap" cs0 as "Hcs0".
     iExtract "Hrmap" cs1 as "Hcs1".
     iExtract "Hrmap" cra as "Hcra".
@@ -501,9 +500,10 @@ Section fundamental.
               is_untrusted_caller := true
            |}).
 
-    iSpecialize ("Hexec" $! _ (frame :: cstk) (W :: Ws) (C :: Cs) with "[]").
+    iSpecialize ("Hexec" with "[]").
     { iPureIntro. apply related_sts_priv_refl_world. }
     iInstr "Hcode".
+    iSpecialize ("Hexec" $! (frame :: cstk) (W :: Ws) (C :: Cs)).
     unfocus_block "Hcode" "Hcls" as "Hcode"; subst hcont.
     rewrite /load_word. iSimpl in "Hcgp".
 
@@ -610,14 +610,13 @@ Section fundamental.
       + iDestruct (big_sepM_lookup with "Hnil") as "%";eauto; simplify_eq.
   Qed.
 
-  Lemma interp_switcher_call (W : WORLD) (C : CmptName) (Nswitcher : namespace)
-    :
+  Lemma interp_switcher_call (W : WORLD) (C : CmptName) (Nswitcher : namespace) :
     na_inv logrel_nais Nswitcher switcher_inv
     ⊢ interp W C (WSentry XSRW_ Local b_switcher e_switcher a_switcher_call).
   Proof.
     iIntros "#Hinv".
     rewrite fixpoint_interp1_eq /=.
-    iIntros "!> %cstk %Ws %Cs %regs %W' _% %".
+    iIntros "!> %regs %W' % %".
     destruct g'; first done.
     iNext ; iApply (interp_expr_switcher_call with "Hinv").
   Qed.
