theories/switcher/switcher_spec_call.v
@@ -4,7 +4,7 @@ From iris.program_logic Require Import weakestpre adequacy lifting.
 From cap_machine Require Import ftlr_base interp_weakening interp_switcher_return.
 From cap_machine Require Import logrel fundamental interp_weakening memory_region rules proofmode monotone.
 From cap_machine Require Import multiple_updates region_invariants_revocation region_invariants_allocation.
-From cap_machine Require Import switcher switcher_preamble.
+From cap_machine Require Export switcher switcher_preamble.
 From stdpp Require Import base.
 From cap_machine Require Import logrel_extra switcher_macros_spec.
 From cap_machine.proofmode Require Import map_simpl register_tactics proofmode.
@@ -533,16 +533,17 @@ Section Switcher.
       iDestruct (big_sepL_sep with "Hstk_val0") as "[_ H]".
       iDestruct (big_sepL_elem_of with "H") as "?"; eauto.
     }
-    iSpecialize ("Hexec" $! _
-                   (frame :: cstk)
-                   ((std_update_multiple W (finz.seq_between a_stk4 e_stk) Temporary) :: Ws)
-                   (C::Cs)
+    iSpecialize ("Hexec" $!
                    (std_update_multiple W (finz.seq_between a_stk4 e_stk) Temporary)
                   with "[]").
     { iPureIntro.
       apply related_sts_pub_priv_world.
       apply related_sts_pub_update_multiple_temp. auto. }
     iInstr "Hcode".
+    iSpecialize ("Hexec" $!
+                   (frame :: cstk)
+                   ((std_update_multiple W (finz.seq_between a_stk4 e_stk) Temporary) :: Ws)
+                   (C::Cs)).
     unfocus_block "Hcode" "Hcls" as "Hcode"; subst hcont.
     rewrite /load_word. iSimpl in "Hcgp".
 
